thys/LTL/example/rewrite_example_poly.sml
@@ -2,11 +2,11 @@
 
 (* Yes, this requires mlton, since mlyacc is distributed with it *)
 (* TODO: Fix this, or have a more generic way to handle it *)
-use "/usr/local/lib/mlton/sml/mlyacc-lib/base.sig";
-use "/usr/local/lib/mlton/sml/mlyacc-lib/join.sml";
-use "/usr/local/lib/mlton/sml/mlyacc-lib/lrtable.sml";
-use "/usr/local/lib/mlton/sml/mlyacc-lib/stream.sml";
-use "/usr/local/lib/mlton/sml/mlyacc-lib/parser2.sml";
+use "/usr/lib/mlton/sml/mlyacc-lib/base.sig";
+use "/usr/lib/mlton/sml/mlyacc-lib/join.sml";
+use "/usr/lib/mlton/sml/mlyacc-lib/lrtable.sml";
+use "/usr/lib/mlton/sml/mlyacc-lib/stream.sml";
+use "/usr/lib/mlton/sml/mlyacc-lib/parser2.sml";
 
 (* Load extracted code *)
 use "rewrite_example.sml";
