thys/LTL/parser/ltl.yacc.sml
@@ -18,55 +18,64 @@ local open LrTable in
 val table=let val actionRows =
 "\
 \\001\000\001\000\011\000\006\000\010\000\007\000\009\000\008\000\008\000\
-\\009\000\007\000\010\000\006\000\013\000\005\000\015\000\004\000\000\000\
-\\001\000\002\000\017\000\003\000\016\000\004\000\015\000\005\000\014\000\
-\\011\000\013\000\012\000\012\000\014\000\029\000\000\000\
-\\001\000\016\000\000\000\000\000\
-\\031\000\002\000\017\000\003\000\016\000\004\000\015\000\005\000\014\000\
-\\011\000\013\000\012\000\012\000\000\000\
-\\032\000\000\000\
-\\033\000\000\000\
-\\034\000\000\000\
-\\035\000\000\000\
+\\009\000\007\000\010\000\006\000\015\000\005\000\017\000\004\000\000\000\
+\\001\000\002\000\019\000\003\000\018\000\004\000\017\000\005\000\016\000\
+\\011\000\015\000\012\000\014\000\013\000\013\000\014\000\012\000\
+\\016\000\033\000\000\000\
+\\001\000\018\000\000\000\000\000\
+\\035\000\002\000\019\000\003\000\018\000\004\000\017\000\005\000\016\000\
+\\011\000\015\000\012\000\014\000\013\000\013\000\014\000\012\000\000\000\
 \\036\000\000\000\
 \\037\000\000\000\
 \\038\000\000\000\
-\\039\000\011\000\013\000\012\000\012\000\000\000\
-\\040\000\011\000\013\000\012\000\012\000\000\000\
-\\041\000\002\000\017\000\003\000\016\000\011\000\013\000\012\000\012\000\000\000\
-\\042\000\002\000\017\000\003\000\016\000\004\000\015\000\011\000\013\000\
-\\012\000\012\000\000\000\
-\\043\000\000\000\
-\\044\000\000\000\
-\\045\000\000\000\
+\\039\000\000\000\
+\\040\000\000\000\
+\\041\000\000\000\
+\\042\000\000\000\
+\\043\000\011\000\015\000\012\000\014\000\013\000\013\000\014\000\012\000\000\000\
+\\044\000\011\000\015\000\012\000\014\000\013\000\013\000\014\000\012\000\000\000\
+\\045\000\002\000\019\000\003\000\018\000\011\000\015\000\012\000\014\000\
+\\013\000\013\000\014\000\012\000\000\000\
+\\046\000\002\000\019\000\003\000\018\000\004\000\017\000\011\000\015\000\
+\\012\000\014\000\013\000\013\000\014\000\012\000\000\000\
+\\047\000\013\000\013\000\014\000\012\000\000\000\
+\\048\000\013\000\013\000\014\000\012\000\000\000\
+\\049\000\000\000\
+\\050\000\000\000\
+\\051\000\000\000\
 \"
 val actionRowNumbers =
 "\000\000\003\000\004\000\000\000\
 \\000\000\000\000\000\000\006\000\
 \\005\000\000\000\000\000\000\000\
 \\000\000\000\000\000\000\000\000\
-\\001\000\010\000\009\000\008\000\
-\\007\000\016\000\015\000\014\000\
-\\013\000\012\000\011\000\017\000\
+\\000\000\000\000\001\000\010\000\
+\\009\000\008\000\007\000\018\000\
+\\017\000\016\000\015\000\014\000\
+\\013\000\012\000\011\000\019\000\
 \\002\000"
 val gotoT =
 "\
-\\001\000\028\000\002\000\001\000\000\000\
+\\001\000\032\000\002\000\001\000\000\000\
 \\000\000\
 \\000\000\
-\\002\000\016\000\000\000\
-\\002\000\017\000\000\000\
 \\002\000\018\000\000\000\
 \\002\000\019\000\000\000\
-\\000\000\
-\\000\000\
 \\002\000\020\000\000\000\
 \\002\000\021\000\000\000\
+\\000\000\
+\\000\000\
 \\002\000\022\000\000\000\
 \\002\000\023\000\000\000\
 \\002\000\024\000\000\000\
 \\002\000\025\000\000\000\
 \\002\000\026\000\000\000\
+\\002\000\027\000\000\000\
+\\002\000\028\000\000\000\
+\\002\000\029\000\000\000\
+\\002\000\030\000\000\000\
+\\000\000\
+\\000\000\
 \\000\000\
 \\000\000\
 \\000\000\
@@ -81,8 +90,8 @@ val gotoT =
 \\000\000\
 \\000\000\
 \"
-val numstates = 29
-val numrules = 15
+val numstates = 33
+val numrules = 17
 val s = ref "" and index = ref 0
 val string_to_int = fn () => 
 let val i = !index
@@ -159,7 +168,7 @@ fn _ => false
 val preferred_change : (term list * term list) list = 
 nil
 val noShift = 
-fn (T 15) => true | _ => false
+fn (T 17) => true | _ => false
 val showTerminal =
 fn (T 0) => "NOT"
   | (T 1) => "OR"
@@ -173,18 +182,20 @@ fn (T 0) => "NOT"
   | (T 9) => "GLOBAL"
   | (T 10) => "UNTIL"
   | (T 11) => "RELEASE"
-  | (T 12) => "LPAREN"
-  | (T 13) => "RPAREN"
-  | (T 14) => "IDENT"
-  | (T 15) => "EOF"
-  | (T 16) => "BAD_CHAR"
+  | (T 12) => "WEAKUNTIL"
+  | (T 13) => "STRONGRELEASE"
+  | (T 14) => "LPAREN"
+  | (T 15) => "RPAREN"
+  | (T 16) => "IDENT"
+  | (T 17) => "EOF"
+  | (T 18) => "BAD_CHAR"
   | _ => "bogus-term"
 local open Header in
 val errtermvalue=
 fn _ => MlyValue.VOID
 end
 val terms : term list = nil
- $$ (T 16) $$ (T 15) $$ (T 13) $$ (T 12) $$ (T 11) $$ (T 10) $$ (T 9) $$ (T 8) $$ (T 7) $$ (T 6) $$ (T 5) $$ (T 4) $$ (T 3) $$ (T 2) $$ (T 1) $$ (T 0)end
+ $$ (T 18) $$ (T 17) $$ (T 15) $$ (T 14) $$ (T 13) $$ (T 12) $$ (T 11) $$ (T 10) $$ (T 9) $$ (T 8) $$ (T 7) $$ (T 6) $$ (T 5) $$ (T 4) $$ (T 3) $$ (T 2) $$ (T 1) $$ (T 0)end
 structure Actions =
 struct 
 exception mlyAction of int
@@ -193,63 +204,71 @@ val actions =
 fn (i392,defaultPos,stack,
     (()):arg) =>
 case (i392,stack)
-of  ( 0, ( ( _, ( MlyValue.formula formula, formula1left, formula1right)) :: rest671)) => let val  result = MlyValue.input ((*#line 36.17 "ltl.yacc"*)formula(*#line 196.1 "ltl.yacc.sml"*)
+of  ( 0, ( ( _, ( MlyValue.formula formula, formula1left, formula1right)) :: rest671)) => let val  result = MlyValue.input ((*#line 38.17 "ltl.yacc"*)formula(*#line 207.1 "ltl.yacc.sml"*)
 )
  in ( LrTable.NT 0, ( result, formula1left, formula1right), rest671)
 end
-|  ( 1, ( ( _, ( MlyValue.IDENT IDENT, IDENT1left, IDENT1right)) :: rest671)) => let val  result = MlyValue.formula ((*#line 38.20 "ltl.yacc"*)Prop_ltlc IDENT(*#line 200.1 "ltl.yacc.sml"*)
+|  ( 1, ( ( _, ( MlyValue.IDENT IDENT, IDENT1left, IDENT1right)) :: rest671)) => let val  result = MlyValue.formula ((*#line 40.41 "ltl.yacc"*)Prop_ltlc IDENT(*#line 211.1 "ltl.yacc.sml"*)
 )
  in ( LrTable.NT 1, ( result, IDENT1left, IDENT1right), rest671)
 end
-|  ( 2, ( ( _, ( _, TRUE1left, TRUE1right)) :: rest671)) => let val  result = MlyValue.formula ((*#line 39.19 "ltl.yacc"*)True_ltlc(*#line 204.1 "ltl.yacc.sml"*)
+|  ( 2, ( ( _, ( _, TRUE1left, TRUE1right)) :: rest671)) => let val  result = MlyValue.formula ((*#line 41.41 "ltl.yacc"*)True_ltlc(*#line 215.1 "ltl.yacc.sml"*)
 )
  in ( LrTable.NT 1, ( result, TRUE1left, TRUE1right), rest671)
 end
-|  ( 3, ( ( _, ( _, FALSE1left, FALSE1right)) :: rest671)) => let val  result = MlyValue.formula ((*#line 40.20 "ltl.yacc"*)False_ltlc(*#line 208.1 "ltl.yacc.sml"*)
+|  ( 3, ( ( _, ( _, FALSE1left, FALSE1right)) :: rest671)) => let val  result = MlyValue.formula ((*#line 42.41 "ltl.yacc"*)False_ltlc(*#line 219.1 "ltl.yacc.sml"*)
 )
  in ( LrTable.NT 1, ( result, FALSE1left, FALSE1right), rest671)
 end
-|  ( 4, ( ( _, ( MlyValue.formula formula, _, formula1right)) :: ( _, ( _, NOT1left, _)) :: rest671)) => let val  result = MlyValue.formula ((*#line 41.25 "ltl.yacc"*)Not_ltlc formula(*#line 212.1 "ltl.yacc.sml"*)
+|  ( 4, ( ( _, ( MlyValue.formula formula, _, formula1right)) :: ( _, ( _, NOT1left, _)) :: rest671)) => let val  result = MlyValue.formula ((*#line 43.41 "ltl.yacc"*)Not_ltlc formula(*#line 223.1 "ltl.yacc.sml"*)
 )
  in ( LrTable.NT 1, ( result, NOT1left, formula1right), rest671)
 end
-|  ( 5, ( ( _, ( MlyValue.formula formula, _, formula1right)) :: ( _, ( _, NEXT1left, _)) :: rest671)) => let val  result = MlyValue.formula ((*#line 42.26 "ltl.yacc"*)Next_ltlc formula(*#line 216.1 "ltl.yacc.sml"*)
+|  ( 5, ( ( _, ( MlyValue.formula formula, _, formula1right)) :: ( _, ( _, NEXT1left, _)) :: rest671)) => let val  result = MlyValue.formula ((*#line 44.41 "ltl.yacc"*)Next_ltlc formula(*#line 227.1 "ltl.yacc.sml"*)
 )
  in ( LrTable.NT 1, ( result, NEXT1left, formula1right), rest671)
 end
-|  ( 6, ( ( _, ( MlyValue.formula formula, _, formula1right)) :: ( _, ( _, FINAL1left, _)) :: rest671)) => let val  result = MlyValue.formula ((*#line 43.27 "ltl.yacc"*)Final_ltlc formula(*#line 220.1 "ltl.yacc.sml"*)
+|  ( 6, ( ( _, ( MlyValue.formula formula, _, formula1right)) :: ( _, ( _, FINAL1left, _)) :: rest671)) => let val  result = MlyValue.formula ((*#line 45.41 "ltl.yacc"*)Final_ltlc formula(*#line 231.1 "ltl.yacc.sml"*)
 )
  in ( LrTable.NT 1, ( result, FINAL1left, formula1right), rest671)
 end
-|  ( 7, ( ( _, ( MlyValue.formula formula, _, formula1right)) :: ( _, ( _, GLOBAL1left, _)) :: rest671)) => let val  result = MlyValue.formula ((*#line 44.28 "ltl.yacc"*)Global_ltlc formula(*#line 224.1 "ltl.yacc.sml"*)
+|  ( 7, ( ( _, ( MlyValue.formula formula, _, formula1right)) :: ( _, ( _, GLOBAL1left, _)) :: rest671)) => let val  result = MlyValue.formula ((*#line 46.41 "ltl.yacc"*)Global_ltlc formula(*#line 235.1 "ltl.yacc.sml"*)
 )
  in ( LrTable.NT 1, ( result, GLOBAL1left, formula1right), rest671)
 end
-|  ( 8, ( ( _, ( MlyValue.formula formula2, _, formula2right)) :: _ :: ( _, ( MlyValue.formula formula1, formula1left, _)) :: rest671)) => let val  result = MlyValue.formula ((*#line 45.31 "ltl.yacc"*)Or_ltlc (formula1, formula2)(*#line 228.1 "ltl.yacc.sml"*)
+|  ( 8, ( ( _, ( MlyValue.formula formula2, _, formula2right)) :: _ :: ( _, ( MlyValue.formula formula1, formula1left, _)) :: rest671)) => let val  result = MlyValue.formula ((*#line 47.41 "ltl.yacc"*)Or_ltlc (formula1, formula2)(*#line 239.1 "ltl.yacc.sml"*)
 )
  in ( LrTable.NT 1, ( result, formula1left, formula2right), rest671)
 end
-|  ( 9, ( ( _, ( MlyValue.formula formula2, _, formula2right)) :: _ :: ( _, ( MlyValue.formula formula1, formula1left, _)) :: rest671)) => let val  result = MlyValue.formula ((*#line 46.33 "ltl.yacc"*)And_ltlc (formula1, formula2)(*#line 232.1 "ltl.yacc.sml"*)
+|  ( 9, ( ( _, ( MlyValue.formula formula2, _, formula2right)) :: _ :: ( _, ( MlyValue.formula formula1, formula1left, _)) :: rest671)) => let val  result = MlyValue.formula ((*#line 48.41 "ltl.yacc"*)And_ltlc (formula1, formula2)(*#line 243.1 "ltl.yacc.sml"*)
 )
  in ( LrTable.NT 1, ( result, formula1left, formula2right), rest671)
 end
-|  ( 10, ( ( _, ( MlyValue.formula formula2, _, formula2right)) :: _ :: ( _, ( MlyValue.formula formula1, formula1left, _)) :: rest671)) => let val  result = MlyValue.formula ((*#line 47.32 "ltl.yacc"*)Implies_ltlc (formula1, formula2)(*#line 236.1 "ltl.yacc.sml"*)
+|  ( 10, ( ( _, ( MlyValue.formula formula2, _, formula2right)) :: _ :: ( _, ( MlyValue.formula formula1, formula1left, _)) :: rest671)) => let val  result = MlyValue.formula ((*#line 49.41 "ltl.yacc"*)Implies_ltlc (formula1, formula2)(*#line 247.1 "ltl.yacc.sml"*)
 )
  in ( LrTable.NT 1, ( result, formula1left, formula2right), rest671)
 end
-|  ( 11, ( ( _, ( MlyValue.formula formula2, _, formula2right)) :: _ :: ( _, ( MlyValue.formula formula1, formula1left, _)) :: rest671)) => let val  result = MlyValue.formula ((*#line 48.35 "ltl.yacc"*)(iff_ltlc formula1 formula2) (*#line 240.1 "ltl.yacc.sml"*)
+|  ( 11, ( ( _, ( MlyValue.formula formula2, _, formula2right)) :: _ :: ( _, ( MlyValue.formula formula1, formula1left, _)) :: rest671)) => let val  result = MlyValue.formula ((*#line 50.41 "ltl.yacc"*)iff_ltlc formula1 formula2(*#line 251.1 "ltl.yacc.sml"*)
 )
  in ( LrTable.NT 1, ( result, formula1left, formula2right), rest671)
 end
-|  ( 12, ( ( _, ( MlyValue.formula formula2, _, formula2right)) :: _ :: ( _, ( MlyValue.formula formula1, formula1left, _)) :: rest671)) => let val  result = MlyValue.formula ((*#line 49.34 "ltl.yacc"*)Until_ltlc (formula1, formula2)(*#line 244.1 "ltl.yacc.sml"*)
+|  ( 12, ( ( _, ( MlyValue.formula formula2, _, formula2right)) :: _ :: ( _, ( MlyValue.formula formula1, formula1left, _)) :: rest671)) => let val  result = MlyValue.formula ((*#line 51.41 "ltl.yacc"*)Until_ltlc (formula1, formula2)(*#line 255.1 "ltl.yacc.sml"*)
 )
  in ( LrTable.NT 1, ( result, formula1left, formula2right), rest671)
 end
-|  ( 13, ( ( _, ( MlyValue.formula formula2, _, formula2right)) :: _ :: ( _, ( MlyValue.formula formula1, formula1left, _)) :: rest671)) => let val  result = MlyValue.formula ((*#line 50.35 "ltl.yacc"*)Release_ltlc (formula1, formula2)(*#line 248.1 "ltl.yacc.sml"*)
+|  ( 13, ( ( _, ( MlyValue.formula formula2, _, formula2right)) :: _ :: ( _, ( MlyValue.formula formula1, formula1left, _)) :: rest671)) => let val  result = MlyValue.formula ((*#line 52.41 "ltl.yacc"*)Release_ltlc (formula1, formula2)(*#line 259.1 "ltl.yacc.sml"*)
 )
  in ( LrTable.NT 1, ( result, formula1left, formula2right), rest671)
 end
-|  ( 14, ( ( _, ( _, _, RPAREN1right)) :: ( _, ( MlyValue.formula formula, _, _)) :: ( _, ( _, LPAREN1left, _)) :: rest671)) => let val  result = MlyValue.formula ((*#line 51.35 "ltl.yacc"*)formula(*#line 252.1 "ltl.yacc.sml"*)
+|  ( 14, ( ( _, ( MlyValue.formula formula2, _, formula2right)) :: _ :: ( _, ( MlyValue.formula formula1, formula1left, _)) :: rest671)) => let val  result = MlyValue.formula ((*#line 53.41 "ltl.yacc"*)WeakUntil_ltlc (formula1, formula2)(*#line 263.1 "ltl.yacc.sml"*)
+)
+ in ( LrTable.NT 1, ( result, formula1left, formula2right), rest671)
+end
+|  ( 15, ( ( _, ( MlyValue.formula formula2, _, formula2right)) :: _ :: ( _, ( MlyValue.formula formula1, formula1left, _)) :: rest671)) => let val  result = MlyValue.formula ((*#line 54.41 "ltl.yacc"*)StrongRelease_ltlc (formula1, formula2)(*#line 267.1 "ltl.yacc.sml"*)
+)
+ in ( LrTable.NT 1, ( result, formula1left, formula2right), rest671)
+end
+|  ( 16, ( ( _, ( _, _, RPAREN1right)) :: ( _, ( MlyValue.formula formula, _, _)) :: ( _, ( _, LPAREN1left, _)) :: rest671)) => let val  result = MlyValue.formula ((*#line 55.41 "ltl.yacc"*)formula(*#line 271.1 "ltl.yacc.sml"*)
 )
  in ( LrTable.NT 1, ( result, LPAREN1left, RPAREN1right), rest671)
 end
@@ -277,10 +296,12 @@ fun FINAL (p1,p2) = Token.TOKEN (ParserData.LrTable.T 8,(ParserData.MlyValue.VOI
 fun GLOBAL (p1,p2) = Token.TOKEN (ParserData.LrTable.T 9,(ParserData.MlyValue.VOID,p1,p2))
 fun UNTIL (p1,p2) = Token.TOKEN (ParserData.LrTable.T 10,(ParserData.MlyValue.VOID,p1,p2))
 fun RELEASE (p1,p2) = Token.TOKEN (ParserData.LrTable.T 11,(ParserData.MlyValue.VOID,p1,p2))
-fun LPAREN (p1,p2) = Token.TOKEN (ParserData.LrTable.T 12,(ParserData.MlyValue.VOID,p1,p2))
-fun RPAREN (p1,p2) = Token.TOKEN (ParserData.LrTable.T 13,(ParserData.MlyValue.VOID,p1,p2))
-fun IDENT (i,p1,p2) = Token.TOKEN (ParserData.LrTable.T 14,(ParserData.MlyValue.IDENT i,p1,p2))
-fun EOF (p1,p2) = Token.TOKEN (ParserData.LrTable.T 15,(ParserData.MlyValue.VOID,p1,p2))
-fun BAD_CHAR (p1,p2) = Token.TOKEN (ParserData.LrTable.T 16,(ParserData.MlyValue.VOID,p1,p2))
+fun WEAKUNTIL (p1,p2) = Token.TOKEN (ParserData.LrTable.T 12,(ParserData.MlyValue.VOID,p1,p2))
+fun STRONGRELEASE (p1,p2) = Token.TOKEN (ParserData.LrTable.T 13,(ParserData.MlyValue.VOID,p1,p2))
+fun LPAREN (p1,p2) = Token.TOKEN (ParserData.LrTable.T 14,(ParserData.MlyValue.VOID,p1,p2))
+fun RPAREN (p1,p2) = Token.TOKEN (ParserData.LrTable.T 15,(ParserData.MlyValue.VOID,p1,p2))
+fun IDENT (i,p1,p2) = Token.TOKEN (ParserData.LrTable.T 16,(ParserData.MlyValue.IDENT i,p1,p2))
+fun EOF (p1,p2) = Token.TOKEN (ParserData.LrTable.T 17,(ParserData.MlyValue.VOID,p1,p2))
+fun BAD_CHAR (p1,p2) = Token.TOKEN (ParserData.LrTable.T 18,(ParserData.MlyValue.VOID,p1,p2))
 end
 end
