thys/LTL/example/Example.thy
@@ -5,12 +5,12 @@
 
 section \<open>Example\<close>
 
-theory LTL_Example
-  imports Main "../LTL" "../LTL_Rewrite" "HOL-Library.Code_Target_Numeral"
+theory Example
+  imports Main "../LTL" "../Rewriting" "HOL-Library.Code_Target_Numeral"
 begin
 
-\<comment> \<open>The included parser always returns a @{typ "String.literal ltlc"}. If a different labelling is 
-  needed one can use @{const ltlc.map_ltlc} to relabel the leafs. In our example we replace the 
+\<comment> \<open>The included parser always returns a @{typ "String.literal ltlc"}. If a different labelling is
+  needed one can use @{const ltlc.map_ltlc} to relabel the leafs. In our example we replace the
   strings by their length.\<close>
 
 definition rewrite :: "String.literal ltlc \<Rightarrow> nat ltln"
